cleanup

Semantics/Imp/Denotational.lean
@@ -10,17 +10,18 @@ From Concrete semantics with Isabelle
 namespace Com
 
 def denote_loop (b: Bexp) (f: State →ˢ State): (State →ˢ State) → (State →ˢ State) :=
-  λ g => Set.ite {s | b s.1} (f ○ g) SFun.id
+  λ g => Set.ite {(s, _) | b s} (f ○ g) SFun.id
 
 def denote: Com → (State →ˢ State)
   | skip₁                  => SFun.id
-  | ass₁ x a               => {s | s.2 = s.1[x ← a s.1]}
+  | ass₁ x a               => {(s, t) | t = s[x ← a s]}
   | cat₁ c d               => c.denote ○ d.denote
-  | if b then c else d end => Set.ite {s | b s.1} c.denote d.denote
+  | if b then c else d end => Set.ite {(s, _) | b s} c.denote d.denote
   | while b loop c end     => Fix.lfp $ denote_loop b c.denote
 
 theorem monotone_denote_loop: monotone (denote_loop b c) :=
-  λ _ _ h => Set.ite_mono _ (SFun.comp_mono PartialOrder.le_rfl h) PartialOrder.le_rfl
+  λ _ _ h =>
+  Set.ite_mono _ (SFun.comp_mono PartialOrder.le_rfl h) PartialOrder.le_rfl
 
 notation (priority := high) "⟦" c "⟧" => denote c
 
@@ -37,11 +38,13 @@ instance equiv: Setoid Com where
     trans := Eq.trans
   }
 
-theorem skipl: (skip₁++c) ≈ c :=
-  by simp only [HasEquiv.Equiv, equiv, denote, SFun.id_comp]
+theorem skipl:
+  (skip₁++c) ≈ c := by
+  simp only [HasEquiv.Equiv, equiv, denote, SFun.id_comp]
 
-theorem skipr: (c++skip₁) ≈ c :=
-  by simp only [HasEquiv.Equiv, equiv, denote, SFun.comp_id]
+theorem skipr:
+  (c++skip₁) ≈ c := by
+  simp only [HasEquiv.Equiv, equiv, denote, SFun.comp_id]
 
 theorem while_unfold:
   while b loop c end ≈ if b then c++ while b loop c end else skip₁ end :=
