Semantics/Imp/Natural.lean
@@ -22,13 +22,14 @@ inductive step: Com × State → State → Prop
   | while₀ₙ {b: Bexp} (hb: b s = false):
     step (while b loop c end, s) s
 
-  | while₁ₙ {b: Bexp} (u: State) (hb: b s = true) (hc: step (c, s) u)
+  | while₁ₙ {b: Bexp}
+    (u: State) (hb: b s = true) (hc: step (c, s) u)
     (hw: step (while b loop c end, u) t):
     step (while b loop c end, s) t
 
-infixl:10 " ⟹ " => step
+infix:10 " ⟹ " => step
 
-private example: (⦃x = 5⦄, s₀) ⟹ (s₀["x" ← 5]) := step.assₙ
+private example: (⦃x = 5⦄, s₀) ⟹ s₀["x" ← 5] := step.assₙ
 
 private example:
    (⦃x = 2; if x <= 1 then y = 3 else z = 4 end⦄, s₀)
@@ -37,21 +38,23 @@ private example:
 
 private example:
   (⦃x = 2; x = 3⦄, s₀) ⟹ s₀["x" ← 3] :=
-  let h1: s₀["x" ← 3] = s₀["x" ← 2]["x" ← 3] := TotalMap.clobber.symm
+  let h1: s₀["x" ← 3] = s₀["x" ← 2]["x" ← 3] :=
+    TotalMap.eval_last.symm
   h1 ▸ step.catₙ _ step.assₙ step.assₙ
 
 /-
 ## Rewriting rules
 -/
 
-theorem skip_eq: ((skip₁, s) ⟹ t) = (s = t) :=
+theorem skip_eq:
+  ((skip₁, s) ⟹ t) = (s = t) :=
   propext {
     mp := λ (step.skipₙ) => rfl,
     mpr := (· ▸ step.skipₙ)
   }
 
 theorem cat_eq:
-  ((c++d, s) ⟹ t) = ∃ w, ((c, s) ⟹ w) ∧ ((d, w) ⟹ t) :=
+  ((c++d, s) ⟹ t) = ∃w, ((c, s) ⟹ w) ∧ ((d, w) ⟹ t) :=
   propext {
     mp := λ (step.catₙ t h1 h2) => ⟨t, h1, h2⟩,
     mpr := λ ⟨w, h1, h2⟩ => step.catₙ w h1 h2
@@ -79,11 +82,12 @@ theorem if_eq':
       | false => λ h => step.if₀ₙ hb h
   }
 
-theorem while_eq: ((while b loop c end, s) ⟹ t) =
-  bif b s then
-    ∃w, ((c, s) ⟹ w) ∧ ((while b loop c end, w) ⟹ t)
-  else
-    s = t :=
+theorem while_eq:
+  ((while b loop c end, s) ⟹ t) =
+    bif b s then
+      ∃w, ((c, s) ⟹ w) ∧ ((while b loop c end, w) ⟹ t)
+    else
+      s = t :=
   propext {
     mp := λ h => match h with
       | step.while₁ₙ t hb hc hw => hb ▸ ⟨t, hc, hw⟩
@@ -105,14 +109,16 @@ instance equiv: Setoid Com where
     trans := λ h1 h2 x n => Iff.trans (h1 x n) (h2 x n)
   }
 
-theorem skipl: (skip₁++c) ≈ c := λ _ _ =>
-  {
+theorem skipl:
+  (skip₁++c) ≈ c :=
+  λ _ _ => {
     mp := λ (step.catₙ _ hc hd) => skip_eq.mp hc ▸ hd,
     mpr := λ h => step.catₙ _ step.skipₙ h
   }
 
-theorem skipr: (c++skip₁) ≈ c := λ _ _ =>
-  {
+theorem skipr:
+  (c++skip₁) ≈ c :=
+  λ _ _ => {
     mp := λ (step.catₙ _ hc hd) => skip_eq.mp hd ▸ hc,
     mpr := λ h => step.catₙ _ h step.skipₙ
   }
@@ -131,7 +137,7 @@ theorem cond_false (h: b ≈ Bexp.false₁):
 
 theorem loop_unfold:
   while b loop c end ≈
-    if b then (c++while b loop c end) else skip₁ end := by
+    if b then c++while b loop c end else skip₁ end := by
   intro s t
   rw [if_eq']
   constructor
@@ -152,7 +158,8 @@ theorem loop_unfold:
 -/
 
 theorem loop_tt (h: b ≈ Bexp.true₁):
-  ¬((while b loop c end, s) ⟹ t) := λ h1 => by
+  ¬((while b loop c end, s) ⟹ t) := by
+  intro h1
   generalize h2: (while b loop c end, s) = p at h1
   induction h1 generalizing s with
   | while₁ₙ _ _ _ _ _ ih2 =>
@@ -172,37 +179,37 @@ theorem loop_tt (h: b ≈ Bexp.true₁):
 -/
 
 theorem deterministic
-  (h1: p ⟹ s) (h2: p ⟹ t): s = t :=
-  by induction h1 generalizing t with
-  | skipₙ => match h2 with | step.skipₙ => rfl
-  | assₙ => match h2 with | step.assₙ => rfl
+  (hps: p ⟹ s) (hpt: p ⟹ t): s = t :=
+  by induction hps generalizing t with
+  | skipₙ => match hpt with | step.skipₙ => rfl
+  | assₙ => match hpt with | step.assₙ => rfl
   | catₙ _ _ _ ihc ihd =>
-    match h2 with
+    match hpt with
     | step.catₙ _ hc hd =>
       exact ihd (ihc hc ▸ hd)
   | if₁ₙ hb _ ih =>
-    match h2 with
+    match hpt with
     | step.if₁ₙ _ hd =>
       exact ih hd
     | step.if₀ₙ hb1 hd =>
       rw [hb] at hb1
       contradiction
   | if₀ₙ hb _ ih =>
-    match h2 with
+    match hpt with
     | step.if₁ₙ hb1 _ =>
       rw [hb] at hb1
       contradiction
     | step.if₀ₙ _ hd =>
       exact ih hd
   | while₁ₙ _ hb _ _ ihc ihw =>
-    match h2 with
+    match hpt with
     | step.while₁ₙ _ _ hc hw =>
       exact ihw (ihc hc ▸ hw)
     | step.while₀ₙ hb1 =>
       rw [hb] at hb1
       contradiction
   | while₀ₙ hb =>
-    match h2 with
+    match hpt with
     | step.while₁ₙ _ hb1 _ _ =>
       rw [hb] at hb1
       contradiction
