Semantics/Maps.lean
@@ -17,19 +17,21 @@ notation m "[" k " ← " v "]" => TotalMap.update m k v
 
 namespace TotalMap
 
-theorem ev: (m[k ← v]) k = v := by
+theorem eval:
+  (m[k ← v]) k = v := by
   unfold TotalMap.update
   rw [beq_self_eq_true, cond_true]
 
-theorem ev_neq (hneq: k != k'):
-    (m[k ← v]) k' = m k' := by
+theorem eval_neq (hneq: k != k'):
+  (m[k ← v]) k' = m k' := by
   unfold TotalMap.update
   rw [bne_iff_ne] at hneq
   rw [Bool.cond_neg]
   rw [beq_eq_false_iff_ne k k']
   exact hneq
 
-theorem clobber: m[k ← v₂][k ← v₁] = m[k ← v₁] := by
+theorem eval_last:
+  m[k ← v₂][k ← v₁] = m[k ← v₁] := by
   funext k'
   match h: k == k' with
   | true =>
@@ -39,7 +41,7 @@ theorem clobber: m[k ← v₂][k ← v₁] = m[k ← v₁] := by
     unfold TotalMap.update
     rw [h, cond_false, cond_false, cond_false]
 
-theorem ev_swap (hneq : k₁ != k₂):
+theorem eval_swap (hneq : k₁ != k₂):
   m[k₂ ← v₂][k₁ ← v₁] = m[k₁ ← v₁][k₂ ← v₂] := by
   funext k'
   match h: k₁ == k' with
@@ -56,7 +58,8 @@ theorem ev_swap (hneq : k₁ != k₂):
     unfold TotalMap.update
     rw [h, cond_false, cond_false]
 
-theorem ev_id: m[k ← m k] = m := by
+theorem eval_id:
+  m[k ← m k] = m := by
   funext k'
   match h: k == k' with
   | true =>
@@ -66,7 +69,8 @@ theorem ev_id: m[k ← m k] = m := by
     unfold TotalMap.update
     rw [h, cond_false]
 
-theorem ev_same: (λ _ => v)[k ← v] = λ _ => v := by
+theorem eval_same:
+  (λ _ => v)[k ← v] = λ _ => v := by
   funext k'
   match h: k == k' with
   | true =>
@@ -77,15 +81,15 @@ theorem ev_same: (λ _ => v)[k ← v] = λ _ => v := by
     rw [h, cond_false]
 
 example (m: TotalMap Nat):
-  m["a" ← 0]["a" ← 2] = m["a" ← 2] := clobber
+  m["a" ← 0]["a" ← 2] = m["a" ← 2] := eval_last
 
 example (m: TotalMap Nat):
   m["a" ← 0]["b" ← 2] = m["b" ← 2]["a" ← 0] := by
-  apply ev_swap
+  apply eval_swap
   simp only [String.reduceBNe]
 
 example (m: TotalMap Nat):
-  m["a" ← m "a"]["b" ← 0] = m["b" ← 0] := ev_id ▸ rfl
+  m["a" ← m "a"]["b" ← 0] = m["b" ← 0] := eval_id ▸ rfl
 
 end TotalMap
 
